opt

pulse/ulib/experimental/Steel.C.Opt.fsti
@@ -1,54 +1,10 @@
 module Steel.C.Opt
+include Steel.ST.C.Opt
 
 module P = FStar.PCM
 open Steel.C.Model.PCM
 open Steel.C.Model.Ref
 open Steel.Effect
-
-/// If no custom PCM is needed, p and q can be instantiated with an all-or-none PCM:
-
-let opt_comp (x y: option 'a): prop = match x, y with
-  | None, _ | _, None -> True
-  | _, _ -> False
-
-let opt_op (x: option 'a) (y: option 'a{opt_comp x y}): option 'a = match x, y with
-  | None, z | z, None -> z
-
-let fstar_opt_pcm #a : P.pcm (option a) = let open P in {
-  p = {composable = opt_comp; op = opt_op; one = None};
-  comm = (fun _ _ -> ());
-  assoc = (fun _ _ _ -> ());
-  assoc_r = (fun _ _ _ -> ());
-  is_unit = (fun _ -> ());
-  refine = (fun x -> Some? x == true);
-}
-
-let opt_pcm #a : pcm (option a) = pcm_of_fstar_pcm fstar_opt_pcm
-
-let option: Type u#a -> Type u#a = option
-
-let none #a: Ghost.erased (option a) = None
-
-[@@__reduce__]
-let some (x: Ghost.erased 'a): Ghost.erased (option 'a) = Some (Ghost.reveal x)
-
-let some_v (x: Ghost.erased (option 'a){Some? x}): Ghost.erased 'a = Some?.v x
-
-val opt_read
-  (#a:Type) (#b:Type) (#x: Ghost.erased b)
-  (r: ref a (opt_pcm #b))
-: Steel b
-    (r `pts_to` Some #b x)
-    (fun _ -> r `pts_to` Some #b x)
-    (requires fun _ -> True)
-    (ensures fun _ x' _ -> Ghost.reveal x == x')
-
-val opt_write
-  (#a:Type) (#b:Type) (#x: Ghost.erased b)
-  (r: ref a (opt_pcm #b)) (y: b)
-: SteelT unit
-    (r `pts_to` Some #b x)
-    (fun _ -> r `pts_to` Some y)
 
 let opt_view
   (a: Type)
@@ -61,53 +17,7 @@ let opt_view
   to_view_frame = (fun x frame -> ());
 }
 
-let exclusive_opt
-  (#a: Type)
-  (x: option a)
-: Lemma
-  (exclusive opt_pcm x <==> ((exists (y: a) . True) ==> Some? x))
-=
-  match x with
-  | None ->
-    if FStar.StrongExcludedMiddle.strong_excluded_middle (exists (y: a). True)
-    then begin
-      let y = FStar.IndefiniteDescription.indefinite_description_ghost a (fun _ -> True) in
-      assert (composable opt_pcm x (Some y))
-    end else begin
-      let phi
-        (frame: option a)
-      : Lemma
-        (frame == None)
-      = match frame with
-        | None -> ()
-        | Some z -> assert (exists (y: a) . True)
-      in
-      Classical.forall_intro phi
-    end
-  | Some _ -> ()
-
-let opt_pcm_fpu
-  (#a: Type)
-  (x: Ghost.erased (option a) { ~ (Ghost.reveal x == one opt_pcm) })
-  (y: a)
-: Tot (frame_preserving_upd opt_pcm x (Some y))
-= base_fpu opt_pcm x (Some y)
-
-val opt_pcm_write
-  (#a:Type) (#b: Type)
-  (r: ref a (opt_pcm #b)) (x: Ghost.erased (option b)) (y: b)
-: Steel unit (r `pts_to` x) (fun _ -> r `pts_to` Some y)
-  (requires (fun _ -> Some? x))
-  (ensures (fun _ _ _ -> True))
-
-val opt_pcm_read
-  (#a:Type) (#b: Type)
-  (r: ref a (opt_pcm #b)) (x: Ghost.erased (option b))
-: Steel b (r `pts_to` x) (fun _ -> r `pts_to` x)
-  (requires (fun _ -> Some? x))
-  (ensures (fun _ y _ -> Ghost.reveal x == Some y))
-
-let opt_read_sel
+val opt_read_sel
   (#a: Type u#0) (#b: Type u#0)
   (r: ref a (opt_pcm #b))
 : Steel b
@@ -118,9 +28,8 @@ let opt_read_sel
     res == h (pts_to_view r (opt_view b)) /\
     res == h' (pts_to_view r (opt_view b))
   ))
-= ref_read_sel r (opt_view b)
 
-let opt_write_sel
+val opt_write_sel
   (#a: Type u#0) (#b: Type u#0)
   (r: ref a (opt_pcm #b))
   (w: b)
@@ -131,14 +40,10 @@ let opt_write_sel
   (ensures (fun _ _ h' ->
     w == h' (pts_to_view r (opt_view b))
   ))
-=
-  let _ = pts_to_view_elim r (opt_view _) in
-  opt_pcm_write r _ w;
-  pts_to_view_intro r _ (opt_view _) w
 
 open Steel.C.Reference
 
-let ref_opt_read
+val ref_opt_read
   (#a: Type u#0) (#b: Type u#0)
   (r: ref a b (opt_pcm #b))
 : Steel b
@@ -149,9 +54,8 @@ let ref_opt_read
     res == h (pts_to_view r (opt_view b)) /\
     res == h' (pts_to_view r (opt_view b))
   ))
-= ref_read_sel r (opt_view b)
 
-let ref_opt_write
+val ref_opt_write
   (#a: Type u#0) (#b: Type u#0)
   (r: ref a b (opt_pcm #b))
   (w: b)
@@ -162,7 +66,6 @@ let ref_opt_write
   (ensures (fun _ _ h' ->
     w == h' (pts_to_view r (opt_view b))
   ))
-= opt_write_sel r w
 
 val malloc
   (#c:Type0) (x: c)
